rt ainvs: new valid_sched_control_inv / valid_refills proofs in progress

proof/invariant-abstract/SchedContextInv_AI.thy
@@ -12,7 +12,7 @@ theory SchedContextInv_AI
 imports "./$L4V_ARCH/ArchIpc_AI"
 begin
 
-text {* invocation related lemmas *}
+text {* valid invocation definitions *}
 
 primrec
   valid_sched_context_inv :: "sched_context_invocation \<Rightarrow> 'z::state_ext state \<Rightarrow> bool"
@@ -44,13 +44,526 @@ where
                  (*  \<and> (mcpriority_tcb_at (\<lambda>mcp. (tcb_priority (the (get_etcb t s))) \<le> mcp)
                                                                       (cur_thread s) s)*)) scptr s))"
 
+
+definition
+  valid_extra_refills :: "nat \<Rightarrow> nat \<Rightarrow> bool"
+where
+  "valid_extra_refills mrefills n \<equiv>
+    mrefills \<le> (n - core_sched_context_bytes) div refill_size_bytes"
+
 primrec
   valid_sched_control_inv :: "sched_control_invocation \<Rightarrow> 'z::state_ext state \<Rightarrow> bool"
 where
     "valid_sched_control_inv (InvokeSchedControlConfigure scptr budget period mrefills badge)
-     = (sc_at scptr and ex_nonz_cap_to scptr
-        (* probably also need something like \<and> mrefills \<le> max_extra_refills *))"
+     = (obj_at (\<lambda>ko. \<exists>sc n. ko = SchedContext sc n \<and> valid_extra_refills mrefills n) scptr
+        and ex_nonz_cap_to scptr and K (MIN_REFILLS \<le> mrefills) (* mrefills = MIN_REFILLS + extra_refills *)
+        and K (budget \<le> us_to_ticks maxTimer_us \<and> budget \<ge> MIN_BUDGET)
+        and K (period \<le> us_to_ticks maxTimer_us \<and> budget \<ge> MIN_BUDGET)
+        and K (budget \<le> period))"
 
+
+text {* refill invariant proofs *}  (* FIXME move? Sporadic_AI? *)
+
+definition valid_refill_amount :: "obj_ref \<Rightarrow> time \<Rightarrow> 'z::state_ext state \<Rightarrow> bool"
+where
+  "valid_refill_amount scptr budget =
+     (obj_at (\<lambda>ko. \<exists>sc n. ko= SchedContext sc n
+      \<and> refills_sum (sc_refills sc) = budget) scptr)"
+
+definition valid_refill_length :: "obj_ref \<Rightarrow> time \<Rightarrow> 'z::state_ext state \<Rightarrow> bool"
+where
+  "valid_refill_length scptr budget =
+     (obj_at (\<lambda>ko. \<exists>sc n. ko= SchedContext sc n
+      \<and> 1 \<le> length (sc_refills sc)
+      \<and> MIN_REFILLS \<le> sc_refill_max sc
+      \<and> length (sc_refills sc) \<le> sc_refill_max sc
+      \<and> (sc_period sc = 0 \<longrightarrow> (sc_refill_max sc = MIN_REFILLS
+                               \<and> length (sc_refills sc) = MIN_REFILLS))) scptr)"
+
+definition valid_refills :: "obj_ref \<Rightarrow> time \<Rightarrow> 'z::state_ext state \<Rightarrow> bool"
+where
+  "valid_refills scptr budget =
+     (obj_at (\<lambda>ko. \<exists>sc n. ko= SchedContext sc n
+      \<and> refills_sum (sc_refills sc) = budget
+      \<and> 1 \<le> length (sc_refills sc)
+      \<and> MIN_REFILLS \<le> sc_refill_max sc
+      \<and> length (sc_refills sc) \<le> sc_refill_max sc
+      \<and> (sc_period sc = 0 \<longrightarrow> (sc_refill_max sc = MIN_REFILLS
+                               \<and> length (sc_refills sc) = MIN_REFILLS))) scptr)"
+
+lemma valid_refills_def2:
+  "valid_refills = (\<lambda>p b. valid_refill_amount p b and valid_refill_length p b)"
+  by (fastforce simp: valid_refills_def valid_refill_amount_def valid_refill_length_def obj_at_def)
+
+definition sc_valid_refills :: "sched_context \<Rightarrow> time \<Rightarrow> bool"
+where
+  "sc_valid_refills sc budget =
+      (refills_sum (sc_refills sc) = budget
+      \<and> 1 \<le> length (sc_refills sc)
+      \<and> MIN_REFILLS \<le> sc_refill_max sc
+      \<and> length (sc_refills sc) \<le> sc_refill_max sc
+      \<and> (sc_period sc = 0 \<longrightarrow> (sc_refill_max sc = MIN_REFILLS
+                               \<and> length (sc_refills sc) = MIN_REFILLS)))"
+
+lemma valid_refills_consumed_time_update[iff]:
+  "valid_refills p b (consumed_time_update f s) = valid_refills p b s"
+  by (simp add: valid_refills_def)
+
+lemma valid_refills_scheduler_action_update[iff]:
+  "valid_refills p b (scheduler_action_update f s) = valid_refills p b s"
+  by (simp add: valid_refills_def)
+
+lemma valid_refills_ready_queues_update[iff]:
+  "valid_refills p b (ready_queues_update f s) = valid_refills p b s"
+  by (simp add: valid_refills_def)
+
+lemma valid_refills_release_queue_update[iff]:
+  "valid_refills p b (release_queue_update f s) = valid_refills p b s"
+  by (simp add: valid_refills_def)
+
+lemma valid_refills_kheap_tcb_update[iff]:
+  "tcb_at t s \<Longrightarrow> valid_refills p b (s\<lparr>kheap := kheap s(t \<mapsto> TCB tcb)\<rparr>) = valid_refills p b s"
+  by (clarsimp simp: valid_refills_def obj_at_def is_tcb)
+
+crunch valid_refills[wp]: tcb_sched_action,set_scheduler_action,refill_capacity,refill_sufficient
+   "valid_refills scp budget"
+crunch valid_refills[wp]: tcb_release_enqueue,tcb_release_remove,refill_ready "valid_refills scp budget"
+  (wp: crunch_wps)
+
+crunch valid_refills[wp]: reschedule_required,
+possible_switch_to "valid_refills scp budget"
+  (wp: dxo_wp_weak hoare_vcg_if_lift2 crunch_wps)
+
+lemma valid_refills_exst [iff]:
+  "valid_refills p b (trans_state f s) = valid_refills p b s"
+  by (simp add: valid_refills_def valid_state_def)
+
+lemma valid_refills_reprogram_timer_update [iff]:
+  "valid_refills p b (reprogram_timer_update f s) = valid_refills p b s"
+  by (simp add: valid_refills_def valid_state_def)
+
+lemma sched_context_resume_valid_refills[wp]:
+  "\<lbrace>valid_refills scptr budget\<rbrace> sched_context_resume scptr \<lbrace>\<lambda>_. valid_refills scptr budget\<rbrace>"
+  by (wpsimp simp: sched_context_resume_def wp: hoare_vcg_if_lift2 hoare_drop_imp)
+
+crunch valid_refills[wp]: sort_queue "valid_refills scp budget"  (wp: mapM_wp')
+
+lemma update_sched_context_valid_refills_no_budget_update:
+  "\<lbrace>valid_refills scptr budget
+     and K (scptr=p \<longrightarrow> sc_valid_refills newsc budget)\<rbrace>
+     update_sched_context p newsc
+      \<lbrace>\<lambda>_. valid_refills scptr budget\<rbrace>"
+  by (wpsimp simp: valid_refills_def update_sched_context_def obj_at_def sc_valid_refills_def
+          wp: set_object_wp get_object_wp)
+
+lemma update_sched_context_valid_refills:
+  "\<lbrace>valid_refills scptr budget
+     and K (1 \<le> length (sc_refills newsc)\<and>MIN_REFILLS \<le> sc_refill_max newsc
+         \<and> length (sc_refills newsc) \<le> sc_refill_max newsc
+         \<and> (sc_period newsc = 0 \<longrightarrow> (sc_refill_max newsc = MIN_REFILLS
+                               \<and> length (sc_refills newsc) = MIN_REFILLS)))\<rbrace>
+     update_sched_context p newsc
+      \<lbrace>\<lambda>_. valid_refills scptr (if p = scptr then refills_sum (sc_refills newsc) else budget)\<rbrace>"
+  apply (wpsimp simp: valid_refills_def update_sched_context_def obj_at_def
+          wp: set_object_wp get_object_wp split_del: if_split)
+  by clarsimp
+
+lemma update_sched_context_valid_refills':
+  "\<lbrace>K (1 \<le> length (sc_refills newsc) \<and> MIN_REFILLS \<le> sc_refill_max newsc
+          \<and> length (sc_refills newsc) \<le> sc_refill_max newsc
+          \<and> (sc_period newsc = 0 \<longrightarrow> (sc_refill_max newsc = MIN_REFILLS
+                               \<and> length (sc_refills newsc) = MIN_REFILLS)))\<rbrace>
+   update_sched_context p newsc  \<lbrace>\<lambda>_. valid_refills p (refills_sum (sc_refills newsc))\<rbrace>"
+  by (wpsimp simp: valid_refills_def update_sched_context_def obj_at_def
+            wp: set_object_wp get_object_wp)
+
+lemma set_thread_state_valid_refills[wp]:
+  "\<lbrace>valid_refills scptr budget\<rbrace> set_thread_state tp st \<lbrace>\<lambda>_. valid_refills scptr budget\<rbrace>"
+  by (wpsimp wp: sts_obj_at_impossible simp: valid_refills_def)
+
+lemma refill_add_tail_valid_refills:
+  "\<lbrace>valid_refills scptr budget\<rbrace> refill_add_tail scptr new \<lbrace>\<lambda>_. valid_refills scptr (budget + (r_amount new))\<rbrace>"
+  apply (wpsimp wp: get_refills_wp get_sched_context_wp set_object_wp get_object_wp
+           simp: refill_add_tail_def set_refills_def update_sched_context_def)
+  by (clarsimp simp: valid_refills_def obj_at_def refills_sum_def)
+
+lemma maybe_add_empty_tail_valid_refills:
+  "\<lbrace>valid_refills scptr budget\<rbrace> maybe_add_empty_tail scptr \<lbrace>\<lambda>_. valid_refills scptr budget\<rbrace>"
+  apply (wpsimp wp: get_refills_wp get_sched_context_wp set_object_wp get_object_wp
+           simp: maybe_add_empty_tail_def refill_add_tail_def is_round_robin_def
+                 set_refills_def update_sched_context_def)
+  by (clarsimp simp: valid_refills_def obj_at_def refills_sum_def)
+
+lemma refill_new_valid_refills[wp]:
+  "\<lbrace>K (MIN_REFILLS \<le> max_refills \<and> (period = 0 \<longrightarrow> max_refills = MIN_REFILLS))\<rbrace>
+    refill_new scptr max_refills budget period \<lbrace>\<lambda>_. valid_refills scptr budget\<rbrace>"
+  apply (wpsimp simp: refill_new_def update_sched_context_def maybe_add_empty_tail_def
+           refill_add_tail_def set_refills_def is_round_robin_def
+            wp:  set_object_wp get_object_wp get_sched_context_wp)
+  by (clarsimp simp: valid_refills_def refills_sum_def obj_at_def MIN_REFILLS_def)
+
+lemma refill_update_valid_refills[wp]:
+  "\<lbrace>K (MIN_REFILLS \<le> new_max_refills \<and> (new_period = 0 \<longrightarrow> new_max_refills = MIN_REFILLS))\<rbrace>
+     refill_update scptr new_period new_budget new_max_refills
+      \<lbrace>\<lambda>_. valid_refills scptr new_budget\<rbrace>"
+  apply (clarsimp simp: refill_update_def)
+  apply (rule hoare_assume_pre)
+  apply (wpsimp simp: update_sched_context_def maybe_add_empty_tail_def refill_add_tail_def
+                      set_refills_def get_refills_def set_object_def is_round_robin_def
+           split_del: if_split
+           wp: get_object_wp get_sched_context_wp hoare_if)
+      apply clarsimp
+      apply (intro conjI impI; clarsimp simp: valid_refills_def obj_at_def refills_sum_def MIN_REFILLS_def)
+     apply clarsimp
+     apply (wpsimp wp: hoare_vcg_all_lift  hoare_vcg_if_lift2 get_sched_context_wp
+               simp: refill_ready_def split_del: if_split)
+    apply wpsimp
+   apply (wpsimp wp: get_sched_context_wp)
+  apply (clarsimp split del: if_split)
+  apply (intro conjI allI impI;
+         clarsimp simp: obj_at_def refills_sum_def valid_refills_def MIN_REFILLS_def
+            split del: if_split)
+  done
+
+lemma sum_list_but_last[iff]:
+  "lista \<noteq> [] \<Longrightarrow> sum_list (map r_amount (butlast lista)) + r_amount (last lista) =
+            sum_list (map r_amount lista)"
+  apply (subgoal_tac "sum_list (map r_amount (butlast lista)) + r_amount (last lista)
+           = sum_list (map r_amount ((butlast lista) @ [last lista]))")
+   apply (drule trans)
+    prefer 2
+    apply simp
+   apply (subst append_butlast_last_id)
+    apply blast+
+  apply (clarsimp simp del:append_butlast_last_id)+
+  done
+
+lemma schedule_used_non_nil:
+  "Suc 0 \<le> length (schedule_used x new)" 
+  by (induct x; clarsimp simp: Let_def)
+
+lemma schedule_used_length':
+  "length (schedule_used x new) = length x \<or> length (schedule_used x new) = length x + 1"
+  by (induct x; clarsimp simp: Let_def)
+
+lemma schedule_used_length:
+  "length (schedule_used x new) =
+   (if ((r_amount new < MIN_BUDGET \<and> 2 \<le> length x) \<or> (x \<noteq> [] \<and> r_time new \<le> r_time (last x)))
+    then length x else length x + 1)"
+  by (induct x; clarsimp simp: Let_def length_greater_0_conv[symmetric] simp del: length_greater_0_conv)
+
+lemma schedule_used_sum [simp]:
+  "refills_sum (schedule_used refills new) = refills_sum (refills @ [new])"
+  apply (induct refills arbitrary: new, simp)
+  apply (clarsimp simp: refills_sum_def Let_def)
+  done
+
+lemma refills_budget_check_pos:
+  "\<lbrakk>refills_budget_check period usage rfls = (t, ls); Suc 0 \<le> length rfls\<rbrakk>
+    \<Longrightarrow> Suc 0 \<le> length ls "
+  apply (induct rfls arbitrary: t ls rule: refills_budget_check.induct)
+   apply simp
+  apply simp
+  apply (clarsimp simp: split: if_split_asm)
+  apply (clarsimp simp add: schedule_used_non_nil)
+  done
+
+lemma valid_refills_sc_update:
+  "(valid_refills p b (s\<lparr>kheap := kheap s(p \<mapsto> SchedContext sc n)\<rparr>))
+       = (sc_valid_refills sc b)"
+  by (clarsimp simp: valid_refills_def obj_at_def sc_valid_refills_def)
+
+
+lemma refill_split_check_valid_refills[wp]: (* applicable only when sc is not round_robin *)
+  "\<lbrace>valid_refills scptr budget
+    and obj_at (\<lambda>ko. \<exists>sc n. ko = SchedContext sc n \<and> sc_period sc \<noteq> 0) scptr\<rbrace>
+      refill_split_check scptr consumed \<lbrace>\<lambda>_. valid_refills scptr budget\<rbrace>"
+  apply (unfold refill_split_check_def)
+  apply (simp add: Let_def set_refills_def update_sched_context_def
+      del: schedule_used.simps split del: if_split)
+  apply (wp  get_refills_wp set_object_wp get_object_wp get_sched_context_wp | wpc )+
+  apply clarify
+  apply (subst valid_refills_sc_update)+
+  apply (intro conjI impI allI; (simp;fail)?)
+    apply (simp add: sc_valid_refills_def valid_refills_def obj_at_def refills_sum_def)
+    apply (case_tac "sc_refills sc"; simp)
+   apply (simp add: sc_valid_refills_def valid_refills_def obj_at_def refills_sum_def Let_def)
+   apply (case_tac "sc_refills sc", simp)
+   apply (case_tac list, simp)
+   apply (case_tac lista; clarsimp)
+  apply (simp add: sc_valid_refills_def valid_refills_def obj_at_def refills_sum_def Let_def)
+  apply (case_tac "sc_refills sc", simp)
+  apply (case_tac list, simp)
+  apply (case_tac lista; clarsimp)
+  done
+
+lemma min_budget_merge_helper:
+   "refills_sum (min_budget_merge b (r0#r1#rs)) = refills_sum (r0#r1#rs)"
+  apply (induction rs arbitrary: r0 r1 b, clarsimp simp: refills_sum_def)
+  apply (clarsimp)
+  apply (drule_tac x="r1\<lparr>r_amount := r_amount r1 + r_amount r0\<rparr>" in meta_spec)
+  apply (drule_tac x=a in meta_spec)
+  apply (clarsimp simp: refills_sum_def)
+ done
+
+lemma min_budget_merge_refills_sum[iff]:
+  "refills_sum (min_budget_merge b refills) = refills_sum refills"
+  apply (cases refills, simp)
+  apply (case_tac list, simp)
+  by (simp only: min_budget_merge_helper)
+
+lemma min_budget_merge_length_helper:
+  "1 \<le> length (min_budget_merge b (r0#r1#rs)) \<and> length (min_budget_merge b (r0#r1#rs)) \<le> length (r0#r1#rs)"
+  apply (induction rs arbitrary: r0 r1 b, simp)
+  apply (clarsimp split del: if_split)
+  apply (drule_tac x="r1\<lparr>r_amount := r_amount r1 + r_amount r0\<rparr>" in meta_spec)
+  apply (drule_tac x=a in meta_spec)
+  by clarsimp
+
+lemma min_budget_merge_length:
+  "1 \<le> length ls \<Longrightarrow> 1 \<le> length (min_budget_merge b ls) \<and> length (min_budget_merge b ls) \<le> length ls"
+  apply (cases ls, simp)
+  apply (case_tac list, simp)
+  by (simp only: min_budget_merge_length_helper)
+
+lemma min_budget_merge_valid_refills:
+  "\<lbrace>valid_refills scptr budget
+    and obj_at (\<lambda>ko. \<exists>n. ko = SchedContext sc n \<and> sc_period sc \<noteq> 0) scptr\<rbrace>
+    set_refills scptr (min_budget_merge full (sc_refills sc)) \<lbrace>\<lambda>_. valid_refills scptr budget\<rbrace>"
+  apply (wpsimp simp: set_refills_def update_sched_context_def set_object_def
+                wp: get_object_wp get_sched_context_wp)
+  apply (clarsimp simp: valid_refills_def obj_at_def)
+  apply (drule min_budget_merge_length[of "sc_refills sc" full, simplified])
+  apply auto
+  done
+
+lemma refill_full_valid_refills[wp]:
+  "\<lbrace>valid_refills scptr budget\<rbrace> refill_full scptr \<lbrace>\<lambda>_. valid_refills scptr budget\<rbrace>"
+  by (wpsimp simp: refill_full_def)
+
+lemma refill_budget_check_valid_refills:
+   "\<lbrace>valid_refills scptr budget
+        and obj_at (\<lambda>ko. \<exists>sc n. ko = SchedContext sc n \<and> sc_period sc \<noteq> 0
+            \<and> (capacity < MIN_BUDGET \<or> length (sc_refills sc) = sc_refill_max sc)) scptr\<rbrace>
+      refill_budget_check scptr usage capacity \<lbrace>\<lambda>_. valid_refills scptr budget\<rbrace>"
+  apply (clarsimp simp: refill_budget_check_def)
+  apply (wpsimp simp: set_refills_def update_sched_context_def set_object_def refill_full_def
+    wp: get_object_wp get_sched_context_wp hoare_drop_imp hoare_vcg_all_lift
+    simp_del: fun_upd_apply)
+  sorry
+
+
+lemma valid_refills_sc_consumed_update[iff]:
+    "valid_refills p b (s\<lparr>kheap := kheap s(p' \<mapsto> SchedContext (sc\<lparr>sc_consumed:=x\<rparr>) n)\<rparr>)
+         = valid_refills p b (s\<lparr>kheap := kheap s(p' \<mapsto> SchedContext sc n)\<rparr>)"
+  by (clarsimp simp: valid_refills_def obj_at_def)
+
+lemma helper: "\<lbrace>valid_refills csc budget
+  and obj_at (\<lambda>ko. ko = SchedContext sc n \<and> refills_sum (sc_refills sc) = budget
+                 \<and> 1 \<le> length (sc_refills sc)) csc\<rbrace>
+        (do robin <- is_round_robin csc;
+            if robin
+            then let new_hd = refill_hd sc\<lparr>r_time := r_time (refill_hd sc) - consumed\<rparr>;
+                     new_tl = refill_tl sc\<lparr>r_time := r_time (refill_tl sc) + consumed\<rparr>
+                 in set_refills csc [new_hd, new_tl]
+            else refill_split_check csc consumed
+         od) \<lbrace>\<lambda>_. valid_refills csc budget\<rbrace>"
+  apply (wpsimp simp: is_round_robin_def set_refills_def update_sched_context_def
+    wp: set_object_wp get_object_wp get_sched_context_wp)
+apply (intro conjI impI allI)
+  apply (clarsimp simp: valid_refills_def obj_at_def refills_sum_def MIN_REFILLS_def)
+  apply (case_tac "sc_refills sc"; clarsimp)
+ apply (case_tac list; clarsimp)
+apply (clarsimp simp: obj_at_def)
+done
+
+lemma commit_time_valid_refills:
+  "\<lbrace>\<lambda>s. valid_refills ptr budget s\<rbrace> commit_time \<lbrace>\<lambda>_ s. valid_refills ptr budget s\<rbrace>"
+  apply (clarsimp simp: commit_time_def)
+  apply (wpsimp simp: update_sched_context_def set_object_def wp: get_object_wp)
+         apply (clarsimp simp: valid_refills_def obj_at_def simp del: fun_upd_apply)
+        apply (wpsimp simp: set_refills_def update_sched_context_def set_object_def
+      wp: get_object_wp get_sched_context_wp)
+         apply (wpsimp wp: hoare_drop_imp hoare_vcg_all_lift)
+  sorry
+
+lemmas valid_refills_kheap_tcb_update'[iff] = valid_refills_kheap_tcb_update[simplified fun_upd_def obj_at_def is_tcb]
+
+lemma thread_set_valid_refills[wp]:
+  "\<lbrace>valid_refills scptr budget\<rbrace> thread_set f tptr \<lbrace>\<lambda>_. valid_refills scptr budget\<rbrace>"
+  apply (wpsimp simp: thread_set_def set_object_def simp_del: fun_upd_apply)
+  apply (clarsimp simp: dest!:get_tcb_SomeD)
+  done
+
+lemma set_simple_ko_valid_refills[wp]:
+  "\<lbrace>valid_refills scptr budget\<rbrace> set_simple_ko C ptr new \<lbrace>\<lambda>_. valid_refills scptr budget\<rbrace>"
+  apply (wpsimp simp: set_simple_ko_def set_object_def partial_inv_def a_type_def
+         wp: get_object_wp simp_del: fun_upd_apply split: kernel_object.splits)
+  apply (intro conjI impI; clarsimp simp: valid_refills_def obj_at_def)
+  done
+
+lemma sc_replies_update_valid_refills[wp]:
+  "\<lbrace>valid_refills scptr budget\<rbrace>
+      set_sc_obj_ref sc_replies_update ptr new \<lbrace>\<lambda>_. valid_refills scptr budget\<rbrace>"
+  apply (wpsimp simp: set_sc_obj_ref_def set_object_def
+         wp: get_object_wp update_sched_context_valid_refills_no_budget_update get_sched_context_wp)
+  apply (clarsimp simp: valid_refills_def obj_at_def sc_valid_refills_def)
+  done
+
+lemma sc_tcb_update_valid_refills[wp]:
+  "\<lbrace>valid_refills scptr budget\<rbrace>
+      set_sc_obj_ref sc_tcb_update ptr new \<lbrace>\<lambda>_. valid_refills scptr budget\<rbrace>"
+  apply (wpsimp simp: set_sc_obj_ref_def set_object_def
+         wp: get_object_wp update_sched_context_valid_refills_no_budget_update get_sched_context_wp)
+  apply (clarsimp simp: valid_refills_def obj_at_def sc_valid_refills_def)
+  done
+
+lemma set_tcb_obj_ref_valid_refills[wp]:
+  "\<lbrace>valid_refills scptr budget\<rbrace>
+      set_tcb_obj_ref f ptr new \<lbrace>\<lambda>_. valid_refills scptr budget\<rbrace>"
+  apply (wpsimp simp: set_tcb_obj_ref_def set_object_def
+         wp: get_object_wp update_sched_context_valid_refills_no_budget_update get_sched_context_wp)
+  apply (clarsimp simp: valid_refills_def obj_at_def sc_valid_refills_def dest!: get_tcb_SomeD)
+  done
+
+crunch valid_refills[wp]: update_sk_obj_ref "valid_refills scp budget"
+ (wp: update_sched_context_valid_refills_no_budget_update simp: )
+
+lemma sched_context_donate_valid_refills[wp]:
+  "\<lbrace>valid_refills scptr budget\<rbrace>
+      sched_context_donate ptr callee \<lbrace>\<lambda>_. valid_refills scptr budget\<rbrace>"
+  apply (wpsimp simp: sched_context_donate_def set_object_def get_sc_obj_ref_def
+         wp: get_object_wp update_sched_context_valid_refills_no_budget_update get_sched_context_wp)
+  done
+
+lemma reply_push_valid_refills[wp]:
+  "\<lbrace>valid_refills scptr budget\<rbrace>
+      reply_push caller callee reply_ptr can_donate \<lbrace>\<lambda>_. valid_refills scptr budget\<rbrace>"
+  apply (wpsimp simp: reply_push_def set_object_def partial_inv_def a_type_def
+              unbind_reply_in_ts_def no_reply_in_ts_def
+         wp: get_object_wp update_sched_context_valid_refills_no_budget_update get_sched_context_wp
+             hoare_drop_imp hoare_vcg_if_lift2 hoare_vcg_all_lift
+         simp_del: fun_upd_apply split: kernel_object.splits)
+  done
+
+crunch valid_refills[wp]: reply_unlink_tcb "valid_refills scp budget"
+ (wp: update_sched_context_valid_refills_no_budget_update gts_inv hoare_drop_imps)
+
+locale SchedContextInv_AI =
+  fixes state_ext_t :: "'state_ext::state_ext itself"
+  fixes some_t :: "'t itself"
+  assumes make_arch_fault_msg_invs[wp]:
+    "\<And>ft t. make_arch_fault_msg ft t \<lbrace>valid_refills scptr budget :: 'state_ext state \<Rightarrow> bool\<rbrace>"
+  assumes lookup_ipc_buffer_valid_refills[wp]:
+    "\<And>t b scptr budget.
+      \<lbrace>valid_refills scptr budget :: 'state_ext state \<Rightarrow> bool\<rbrace>
+        lookup_ipc_buffer b t
+      \<lbrace>\<lambda>_. valid_refills scptr budget\<rbrace>"
+
+lemma as_user_valid_refills[wp]:
+  "\<lbrace>valid_refills scptr budget\<rbrace>
+      as_user t f \<lbrace>\<lambda>_. valid_refills scptr budget\<rbrace>"
+  apply (clarsimp simp: as_user_def split_def)
+  apply (wpsimp wp: select_f_wp set_object_wp)
+  by (clarsimp dest!: get_tcb_SomeD simp: valid_refills_def obj_at_def)
+
+crunch valid_refills[wp]: set_message_info "valid_refills scp budget"
+crunch valid_refills[wp]: set_cdt,set_original,set_extra_badge "valid_refills scp budget"
+  (simp: valid_refills_def)
+
+
+lemma set_cap_valid_refills [wp]:
+ "\<lbrace>valid_refills scp budget\<rbrace> set_cap c p \<lbrace>\<lambda>rv. valid_refills scp budget\<rbrace>"
+  apply (simp add: set_cap_def split_def)
+  apply (wpsimp simp: set_object_def wp: get_object_wp)
+  apply (fastforce simp: valid_refills_def obj_at_def)
+  done
+
+crunch valid_refills[wp]: cap_insert "valid_refills scp budget"
+  (wp: hoare_drop_imps)
+
+lemma dmo_storeWord_valid_refills[wp]:
+  "\<lbrace>valid_refills scp budget\<rbrace> do_machine_op (storeWord x y) \<lbrace>\<lambda>_. valid_refills scp budget\<rbrace>"
+  by (simp add: do_machine_op_def valid_refills_def |  wp | wpc)+
+
+lemma sched_context_update_consumed_valid_refills [wp]:
+ "\<lbrace>valid_refills scp budget\<rbrace> sched_context_update_consumed scptr \<lbrace>\<lambda>rv. valid_refills scp budget\<rbrace>"
+  apply (simp add: sched_context_update_consumed_def)
+  apply (wpsimp simp: set_object_def
+      wp: get_object_wp update_sched_context_valid_refills_no_budget_update get_sched_context_wp)
+  apply (clarsimp simp: valid_refills_def obj_at_def sc_valid_refills_def)
+  done
+
+lemma set_mrs_valid_refills [wp]:
+ "\<lbrace>valid_refills scp budget\<rbrace> set_mrs thread buf msgs \<lbrace>\<lambda>rv. valid_refills scp budget\<rbrace>"
+  apply (simp add: set_mrs_def split_def)
+  apply (wpsimp simp: set_object_def zipWithM_x_mapM_x wp: get_object_wp mapM_x_wp' split_del: if_split)
+  apply (clarsimp simp: valid_refills_def obj_at_def get_tcb_SomeD)
+  done
+
+crunch valid_refills[wp]: copy_mrs "valid_refills scp budget"
+  (wp: mapM_wp')
+
+lemma transfer_caps_loop_valid_refills[wp]:
+  "\<And>ep buffer n caps slots mi.
+    \<lbrace>valid_refills scp budget\<rbrace>
+      transfer_caps_loop ep buffer n caps slots mi
+    \<lbrace>\<lambda>rv. valid_refills scp budget\<rbrace>"
+  by (wp transfer_caps_loop_pres cap_insert_valid_refills)
+
+context SchedContextInv_AI begin
+
+crunch valid_refills[wp]: do_ipc_transfer "valid_refills scp budget :: 'state_ext state \<Rightarrow> bool"
+
+end
+
+locale SchedContextInv_AI2 = SchedContextInv_AI state_ext_t some_t
+  for state_ext_t :: "'state_ext::state_ext itself" and some_t :: "'t itself"+
+  assumes  send_ipc_valid_refills[wp]:
+  "\<lbrace>valid_refills scptr budget\<rbrace> send_ipc block call badge can_grant can_donate thread epptr
+      \<lbrace>\<lambda>_. valid_refills scptr budget\<rbrace>"
+
+context SchedContextInv_AI2 begin
+crunch valid_refills[wp]: handle_timeout "valid_refills scp budget"
+
+lemma end_timeslice_valid_refills[wp]:
+  "\<lbrace>valid_refills scptr budget\<rbrace> end_timeslice canTimeout \<lbrace>\<lambda>_. valid_refills scptr budget\<rbrace>"
+  apply (clarsimp simp: end_timeslice_def)
+  by (wpsimp simp: end_timeslice_def wp: hoare_drop_imps split_del: if_split)
+
+lemma charge_budget_valid_refills[wp]:
+  "\<lbrace>valid_refills scptr budget\<rbrace> charge_budget capacity consumed canTimeout \<lbrace>\<lambda>_. valid_refills scptr budget\<rbrace>"
+  apply (clarsimp simp: charge_budget_def)
+  apply (wpsimp wp: update_sched_context_valid_refills_no_budget_update get_sched_context_wp get_object_wp
+          get_refills_wp hoare_drop_imp hoare_vcg_all_lift simp_del: fun_upd_apply
+           simp: Let_def set_refills_def update_sched_context_def set_object_def is_round_robin_def
+          refill_budget_check_def refill_full_def refill_split_check_def)
+  apply (clarsimp simp: valid_refills_def obj_at_def MIN_REFILLS_def)
+  sorry
+
+lemma check_budget_valid_refills[wp]:
+  "\<lbrace>valid_refills scptr budget\<rbrace> check_budget \<lbrace>\<lambda>_. valid_refills scptr budget\<rbrace>"
+  apply (clarsimp simp: check_budget_def)
+  by (wpsimp simp: is_round_robin_def refill_full_def refill_size_def refill_capacity_def
+    wp: get_sched_context_wp get_refills_wp)
+
+
+lemma
+  "\<lbrace>valid_refills scptr budget and
+   valid_sched_control_inv (InvokeSchedControlConfigure scptr budget period mrefills badge)\<rbrace>
+   invoke_sched_control_configure (InvokeSchedControlConfigure scptr budget period mrefills badge)
+   \<lbrace>\<lambda>_. valid_refills scptr budget\<rbrace>"
+  apply (clarsimp simp: invoke_sched_control_configure_def)
+  apply (rule conjI;
+      wpsimp simp: invoke_sched_control_configure_def split_def cong: if_cong conj_cong
+             wp: hoare_vcg_if_lift2 get_sched_context_wp commit_time_valid_refills
+                 hoare_drop_imp update_sched_context_valid_refills_no_budget_update
+            split_del: if_split)
+  by (clarsimp simp: valid_refills_def sc_valid_refills_def obj_at_def MIN_REFILLS_def refills_sum_def)+
+
+end
+
+text {* invocation related lemmas *}
 
 lemma sched_context_bind_tcb_typ_at[wp]:
   "\<lbrace>\<lambda>s. P (typ_at T p s)\<rbrace>
@@ -190,32 +703,6 @@ lemma end_timeslice_invs:
     apply (case_tac "tcb_state tcb"; simp)
    apply simp
   done
-thm refill_budget_check_def
-
-lemma schedule_used_non_nil:
-  "Suc 0 \<le> length (schedule_used x new)" 
-  by (induct x; clarsimp simp: Let_def)
-
-lemma schedule_used_Cons:
-  "\<exists>r rs. schedule_used x new = r#rs"
-  by (induct x; clarsimp simp: Let_def)
-
-lemma refills_budget_check_pos:
-  "\<lbrakk>refills_budget_check period usage rfls = (t, ls); Suc 0 \<le> length rfls\<rbrakk>
-    \<Longrightarrow> Suc 0 \<le> length ls "
-  apply (induct rfls arbitrary: t ls rule: refills_budget_check.induct)
-   apply simp
-  apply simp
-  apply (clarsimp simp: split: if_split_asm)
-  apply (clarsimp simp add: schedule_used_non_nil)
-  done
-
-lemma min_budget_check_pos: "Suc 0 \<le> length refills \<Longrightarrow> Suc 0\<le> length (min_budget_merge full refills)"
-(* in the C code, this comes at the end of refill_budget_check, where it says
-        /* this loop is guaranteed to terminate as the sum of
-         * rAmount in a refill must be >= MIN_BUDGET */
-we need to prove this. *)
-  sorry
 
 lemma invs_valid_refills:
   "\<lbrakk> invs s; ko_at (SchedContext sc n) scptr s\<rbrakk> \<Longrightarrow> Suc 0 \<le> length (sc_refills sc)"
@@ -223,46 +710,38 @@ lemma invs_valid_refills:
 
 lemma refill_budget_check_invs:
   "\<lbrace>invs\<rbrace> refill_budget_check sc_ptr usage capacity \<lbrace>\<lambda>rv. invs\<rbrace>"
-apply (clarsimp simp: refill_budget_check_def)
-
-   apply_trace (wpsimp simp: refill_budget_check_def refill_full_def
-                refill_size_def split_def
-          wp: get_sched_context_wp static_imp_wp
-              hoare_vcg_all_lift hoare_vcg_if_lift2)
-apply (wpsimp wp: get_refills_wp)
-apply (wpsimp wp: get_sched_context_wp)
-apply (wpsimp wp: hoare_drop_imp)
-apply (wpsimp wp: hoare_drop_imp hoare_vcg_all_lift)
-apply (wpsimp wp: hoare_vcg_if_lift2 hoare_drop_imp hoare_vcg_conj_lift split_del: if_split)
-apply wpsimp
-apply (wpsimp simp: wp: hoare_vcg_all_lift hoare_drop_imp)
-apply (wpsimp wp: get_refills_wp)
-apply wpsimp+
-apply (wpsimp simp: refill_full_def refill_size_def)
-apply (wpsimp wp: get_refills_wp)
-apply wpsimp+
-apply (wpsimp wp: get_sched_context_wp simp: refill_full_def refill_size_def)
-sorry
+  apply (clarsimp simp: refill_budget_check_def)
+  apply (wpsimp simp: refill_budget_check_def refill_full_def
+      refill_size_def split_def
+      wp: get_sched_context_wp static_imp_wp hoare_drop_imp
+      hoare_vcg_all_lift hoare_vcg_if_lift2 split_del: if_split)
+  apply (drule invs_valid_objs)
+  apply (drule_tac sc=sc in valid_sched_context_objsI)
+   apply (clarsimp simp: obj_at_def, assumption)
+  apply (intro conjI impI allI; (clarsimp; intro conjI impI)?)
+             apply (clarsimp simp: Let_def)
+            apply (clarsimp simp: Let_def valid_sched_context_def dest!: refills_budget_check_pos split: if_split_asm)
+  sorry
 
 
-thm charge_budget_def check_budget_def
 lemma charge_budget_invs: "\<lbrace>invs\<rbrace> charge_budget capacity consumed canTimeout \<lbrace>\<lambda>rv. invs\<rbrace>"
-apply (clarsimp simp: charge_budget_def)
-apply (wpsimp wp: end_timeslice_invs gts_wp get_object_wp get_sched_context_wp
-hoare_drop_imp get_refills_wp hoare_vcg_all_lift refill_budget_check_invs
- simp: update_sched_context_def set_object_def Let_def set_refills_def)
-sorry
+  apply (clarsimp simp: charge_budget_def)
+  apply (wpsimp wp: end_timeslice_invs gts_wp get_object_wp get_sched_context_wp
+      hoare_drop_imp get_refills_wp hoare_vcg_all_lift refill_budget_check_invs
+      simp: update_sched_context_def set_object_def Let_def set_refills_def)
+  sorry
 
 lemma check_budget_invs: "\<lbrace>invs\<rbrace> check_budget \<lbrace>\<lambda>rv. invs\<rbrace>"
     by (wpsimp simp: check_budget_def refill_full_def refill_size_def
             wp: get_refills_inv hoare_drop_imp get_sched_context_wp charge_budget_invs)
 
 crunch invs[wp]: tcb_release_remove invs
-thm invoke_sched_control_configure_def check_budget_def
+
 lemma invoke_sched_control_configure_invs[wp]:
   "\<lbrace>invs and valid_sched_control_inv i\<rbrace> invoke_sched_control_configure i \<lbrace>\<lambda>rv. invs\<rbrace>"
   by (cases i;
-     wpsimp simp: invoke_sched_control_configure_def valid_sched_control_inv_def refill_update_def
+     wpsimp simp: invoke_sched_control_configure_def valid_sched_control_inv_def 
+                  refill_update_def update_sched_context_def
       split_del: if_split
       wp: commit_time_invs update_sc_badge_invs hoare_vcg_if_lift2 check_budget_invs
          hoare_drop_imp get_sched_context_wp charge_budget_invs)
@@ -308,7 +787,7 @@ lemma sts_valid_sched_context_inv:
 
 lemma sts_valid_sched_control_inv:
   "\<lbrace>valid_sched_control_inv sci\<rbrace> set_thread_state t st \<lbrace>\<lambda>rv. valid_sched_control_inv sci\<rbrace>"
-  by (cases sci; wpsimp)
+  by (cases sci; wpsimp simp: obj_at_def  get_tcb_rev wp: sts_obj_at_impossible)
 
 lemma decode_sched_context_inv_inv:
   "\<lbrace>P\<rbrace>
@@ -397,9 +876,12 @@ lemma decode_sched_control_inv_wf:
   apply (erule ballE[where x="hd excaps"])
    prefer 2
    apply (drule hd_in_set, simp)
-  apply (fastforce simp add: valid_cap_def obj_at_def split: cap.split_asm)
-  done
-
+  apply (clarsimp simp add: valid_cap_def obj_at_def is_sc_obj_def
+ split: cap.split_asm)
+apply (case_tac ko; simp)
+apply (clarsimp simp: valid_extra_refills_def refill_absolute_max_def MachineOps.us_to_ticks_mono
+not_less MIN_BUDGET_def MIN_BUDGET_US_def ARM.kernelWCET_ticks_def)
+sorry (* need us_to_ticks to be monotonic and some more *)
 
 
 
